update invariant and sketch proof till comp_Return

compiler/backend/proofs/word_to_stackProofScript.sml
@@ -855,16 +855,24 @@ End
   f' is the size of the current frame
   lens tracks the size of each remaining stack frame on the stackLang stack
 *)
-(* TODO define this
-    (!sm. s.stack_max = SOME sm ==>
-    LENGTH t.stack - t.stack_space - f <= sm /\
-    IS_SOME s.locals_size /\
-    (?ss. stack_size s.stack = SOME ss /\
-    ss = LENGTH t.stack - t.stack_space - f))
-*)
+
+(* Stack size as predicted by the wordLang state is a conservative estimate of the
+   actual stack usage. *)
+Definition stack_size_rel_def:
+  stack_size_rel f s_locals_size s_stack_limit s_stack_max s_stack
+    t_stack t_stack_space (extra : num) ⇔
+    (f ≠ 0 ==> the f s_locals_size = f) ∧
+    s_stack_limit = LENGTH t_stack ∧
+    ∀sm. s_stack_max = SOME sm ⇒
+      LENGTH t_stack - t_stack_space - f - extra ≤ sm ∧
+      IS_SOME s_locals_size ∧
+      (?ss. stack_size s_stack = SOME ss ∧
+        ss = LENGTH t_stack - t_stack_space - f - extra)
+End
 
 Definition state_rel_def:
-  state_rel ac k f f' (s:('a,num # 'c,'ffi) wordSem$state) (t:('a,'c,'ffi) stackSem$state) lens ⇔
+  state_rel ac k f f' (s:('a,num # 'c,'ffi) wordSem$state)
+    (t:('a,'c,'ffi) stackSem$state) lens extra ⇔
     (s.clock = t.clock) /\ (s.gc_fun = t.gc_fun) /\ (s.permute = K I) /\
     (t.ffi = s.ffi) /\ t.use_stack /\ t.use_store /\ t.use_alloc /\
     (t.memory = s.memory) /\ (t.mdomain = s.mdomain) /\ 4 < k /\
@@ -909,17 +917,9 @@ Definition state_rel_def:
     t.stack_space + f <= LENGTH t.stack /\ LENGTH t.stack < dimword (:'a) /\
     (if f' = 0 then f = 0 else (f = f' + 1)) /\
     wf s.locals /\
-    (* Stack size as predicted by the wordLang state is a conservative estimate of the
-       actual stack usage. *)
-    (f <> 0 ==> the f s.locals_size = f) /\
-    s.stack_limit = LENGTH t.stack /\
-(*
-    LENGTH t.stack - t.stack_space - f <= the (LENGTH t.stack - t.stack_space - f) s.stack_max /\
-    (IS_SOME s.stack_max ==> IS_SOME (stack_size s.stack)) /\
-    (IS_SOME s.stack_max ==> IS_SOME s.locals_size) /\
-    (IS_SOME s.stack_max ==> the (LENGTH t.stack - t.stack_space - f) (stack_size s.stack) = LENGTH t.stack - t.stack_space - f) /\
-*)
-    let stack = DROP t.stack_space t.stack in
+    stack_size_rel f s.locals_size s.stack_limit s.stack_max s.stack
+      t.stack t.stack_space (extra : num) ∧
+    let stack = DROP (t.stack_space + extra) t.stack in
     (*First f things on stack are the live stack vars*)
     let current_frame = TAKE f stack in
     let rest_of_stack = DROP f stack in
@@ -933,7 +933,6 @@ Definition state_rel_def:
              n DIV 2 < k + f')
 End
 
-(*TODO all the state_rel stuff should go here.*)
 (* correctness proof *)
 
 Triviality evaluate_SeqStackFree:
@@ -958,7 +957,6 @@ val convs_def = LIST_CONJ
    wordLangTheory.every_var_imm_def,
    wordLangTheory.every_stack_var_def,
    wordLangTheory.every_name_def]
-
 
 (*
 Triviality LENGTH_write_bitmap:
@@ -1353,14 +1351,15 @@ Theorem evaluate_wLive[local]:
   wLive names (bs,n) (k,f,f') = (wlive_prog,(bs',n')) /\
   (∀x. x ∈ domain (FST names) ⇒ EVEN x /\ k ≤ x DIV 2) /\
   (∀x. x ∈ domain (SND names) ⇒ EVEN x /\ k ≤ x DIV 2) /\
-  state_rel ac k f f' (s:('a,num # 'c,'ffi) wordSem$state) t lens /\ 1 <= f /\
+  state_rel ac k f f' (s:('a,num # 'c,'ffi) wordSem$state) t lens 0 /\
+  1 <= f /\
   (cut_envs names s.locals = SOME envs) /\
   LENGTH (append bs) ≤ n ∧ n - LENGTH (append bs) ≤ LENGTH t.bitmaps ∧
   isPREFIX (append bs') (DROP (n - LENGTH (append bs)) t.bitmaps) ==>
   ?t5:('a,'c,'ffi) stackSem$state bs5.
     (evaluate (wlive_prog,t) = (NONE,t5)) /\
-    state_rel ac k 0 0 (push_env envs ^nn s with <|locals := LN; locals_size := SOME 0|>) t5 (f'::lens) /\
-    state_rel ac k f f' s t5 lens /\
+    state_rel ac k 0 0 (push_env envs ^nn s with <|locals := LN; locals_size := SOME 0|>) t5 (f'::lens) 0 /\
+    state_rel ac k f f' s t5 lens 0 /\
     LENGTH t5.stack = LENGTH t.stack /\ t5.stack_space = t.stack_space /\
     !i. i ≠ k ==> get_var i t5 = get_var i t
 Proof
@@ -1392,172 +1391,172 @@ Proof
     \\ match_mp_tac (GSYM DROP_list_LUPDATE_IGNORE |> Q.SPEC `[x]`
            |> SIMP_RULE std_ss [list_LUPDATE_def])
     \\ fsrw_tac[] [] \\ decide_tac)
-  >~[`flat_exp_conventions`]
+  >>~[`flat_exp_conventions word_prog`]
   >- metis_tac[]
-  >~[`post_alloc_conventions`]
   >- metis_tac[]
-  >~[`_ ≤ _ + the _ _`]
+  >>~[`post_alloc_conventions k word_prog`]
+  >- metis_tac[]
+  >- metis_tac[]
+  >~[`stack_rel k s.handler _ _ _ _ _ (f'::lens)`]
   >- (
-    rw[OPTION_MAP2_DEF,IS_SOME_EXISTS,MAX_DEF] >>
-    fs[the_eqn,stack_size_eq] >> fs[])
-  >~ [`the (_ - _) _ = _ - t.stack_space`]
-  >- (
-    fs[IS_SOME_EXISTS,OPTION_MAP2_DEF,PULL_EXISTS] >> fs[] >>
-    fs[the_eqn,CaseEq"option",stack_size_eq] >>
-    rveq >> fs[])
-  >~[`IS_SOME (stack_size (_::s.stack))`]
-  >- fs[OPTION_MAP2_DEF,IS_SOME_EXISTS,MAX_DEF,the_eqn,CaseEq"option",stack_size_eq]
-  >~[`flat_exp_conventions pp`]
-  >- metis_tac[]
-  >~[`post_alloc_conventions k pp`]
-  >- metis_tac[]
-  \\ fsrw_tac[][wf_def]
-  \\ fsrw_tac[] [stack_rel_def,stack_rel_aux_def,abs_stack_def]
-  \\ Cases_on `DROP t.stack_space t.stack` \\ fsrw_tac[] []
-  \\ fsrw_tac[] [LUPDATE_def,abs_stack_def]
-  \\ conj_tac
-  >- (
-    Q.ISPEC_THEN `SND envs` mp_tac  env_to_list_K_I_IMP
-    \\ fsrw_tac[] [env_to_list_def,sorted_env_def,LET_DEF] \\ srw_tac[] []
-    \\ `s.permute 0 = I` by fsrw_tac[] [FUN_EQ_THM] \\ fsrw_tac[] [])
-  \\ fsrw_tac[] [full_read_bitmap_def,GSYM word_add_n2w]
-  \\ `i < dimword(:α) ∧ (i+1) MOD dimword(:'a) ≠ 0` by (
-      fs[insert_bitmap_def] >> rveq>>
+    fsrw_tac[][wf_def]
+    \\ fsrw_tac[] [stack_rel_def,stack_rel_aux_def,abs_stack_def]
+    \\ Cases_on `DROP t.stack_space t.stack` \\ fsrw_tac[] []
+    \\ fsrw_tac[] [LUPDATE_def,abs_stack_def]
+    \\ conj_tac
+    >- (
+      Q.ISPEC_THEN `SND envs` mp_tac  env_to_list_K_I_IMP
+      \\ fsrw_tac[] [env_to_list_def,sorted_env_def,LET_DEF] \\ srw_tac[] []
+      \\ `s.permute 0 = I` by fsrw_tac[] [FUN_EQ_THM] \\ fsrw_tac[] [])
+    \\ fsrw_tac[] [full_read_bitmap_def,GSYM word_add_n2w]
+    \\ `i < dimword(:α) ∧ (i+1) MOD dimword(:'a) ≠ 0` by (
+        fs[insert_bitmap_def] >> rveq>>
+        drule IS_PREFIX_LENGTH>>
+        simp[])
+    \\ drule (GEN_ALL read_bitmap_insert_bitmap |> INST_TYPE [beta |-> alpha])
+    \\ simp[IS_SOME_EXISTS,PULL_EXISTS]
+    \\ ONCE_REWRITE_TAC[CONJ_COMM]
+    \\ qpat_x_assum `insert_bitmap _ _ = _` mp_tac
+    \\ `n = LENGTH (TAKE (n-LENGTH (append bs)) t.bitmaps) + LENGTH (append bs)` by fs[LENGTH_TAKE]
+    \\ pop_assum SUBST1_TAC
+    \\ strip_tac
+    \\ disch_then drule
+    \\ simp[read_bitmap_write_bitmap]
+    \\ strip_tac
+    \\ `isPREFIX (DROP i (TAKE (n − LENGTH (append bs)) t.bitmaps ++ append bs')) (DROP i t.bitmaps)` by (
+      fs[LENGTH_TAKE,insert_bitmap_def]>>rveq>>fs[]>>
+      qmatch_goalsub_abbrev_tac`DROP a b`>>
+      `DROP a b = write_bitmap (SND names) k f'` by
+        (unabbrev_all_tac>> simp[DROP_APPEND])>>
+      drule isPREFIX_DROP>>
+      disch_then(qspec_then`LENGTH (append bs)` mp_tac)>>
+      simp[DROP_APPEND,DROP_LENGTH_NIL]>>
+      simp[Abbr`a`]>>
+      DEP_REWRITE_TAC[DROP_DROP,LENGTH_TAKE]>>
+      simp[]>>
       drule IS_PREFIX_LENGTH>>
       simp[])
-  \\ drule (GEN_ALL read_bitmap_insert_bitmap |> INST_TYPE [beta |-> alpha])
-  \\ simp[IS_SOME_EXISTS,PULL_EXISTS]
-  \\ ONCE_REWRITE_TAC[CONJ_COMM]
-  \\ qpat_x_assum `insert_bitmap _ _ = _` mp_tac
-  \\ `n = LENGTH (TAKE (n-LENGTH (append bs)) t.bitmaps) + LENGTH (append bs)` by fs[LENGTH_TAKE]
-  \\ pop_assum SUBST1_TAC
-  \\ strip_tac
-  \\ disch_then drule
-  \\ simp[read_bitmap_write_bitmap]
-  \\ strip_tac
-  \\ `isPREFIX (DROP i (TAKE (n − LENGTH (append bs)) t.bitmaps ++ append bs')) (DROP i t.bitmaps)` by (
-    fs[LENGTH_TAKE,insert_bitmap_def]>>rveq>>fs[]>>
-    qmatch_goalsub_abbrev_tac`DROP a b`>>
-    `DROP a b = write_bitmap (SND names) k f'` by
-      (unabbrev_all_tac>> simp[DROP_APPEND])>>
-    drule isPREFIX_DROP>>
-    disch_then(qspec_then`LENGTH (append bs)` mp_tac)>>
-    simp[DROP_APPEND,DROP_LENGTH_NIL]>>
-    simp[Abbr`a`]>>
-    DEP_REWRITE_TAC[DROP_DROP,LENGTH_TAKE]>>
-    simp[]>>
-    drule IS_PREFIX_LENGTH>>
-    simp[])
-  \\ fsrw_tac[][IS_PREFIX_APPEND]
-  \\ imp_res_tac read_bitmap_append_extra
-  \\ simp[DROP_APPEND]
-  \\ gvs[]
-  \\ ntac 2 (pop_assum kall_tac)
-  \\ conj_tac
-  >- (
-    srw_tac[][]
-    \\ imp_res_tac abs_stack_IMP_LENGTH
-    \\ Cases_on`s.handler<LENGTH s.stack`>>fsrw_tac[][]
-    \\ qpat_x_assum`is_handler_frame _`mp_tac
-    >- (simp[ADD1,EL_CONS,PRE_SUB1,LASTN_CONS])
-    \\ simp[ADD1]
-    \\ `LENGTH s.stack - s.handler = 0` by DECIDE_TAC
-    \\ simp[is_handler_frame_def])
-  \\ simp[stack_rel_aux_def]
-  \\ `∀x. s.permute x = I` by simp[FUN_EQ_THM]
-  \\ simp[list_rearrange_I]
-  \\ qmatch_assum_abbrev_tac`DROP nn ll = _`
-  \\ qispl_then[`nn`,`ll`]mp_tac LENGTH_DROP
-  \\ asm_simp_tac(std_ss)[Abbr`ll`,Abbr`nn`]
-  \\ simp[]
-  \\ rpt strip_tac
-  >- (
-    qpat_x_assum`cut_envs _ _ = SOME _` mp_tac>>
-    simp[cut_envs_def,cut_names_def,AllCaseEqs()]>>
-    rw[]>>
-    gvs[ALOOKUP_toAList,lookup_inter,AllCaseEqs(),domain_lookup]>>
-    last_x_assum drule>>
-    strip_tac>>
-    first_x_assum drule>>
-    simp[]>>
-    strip_tac>>
-    DEP_REWRITE_TAC[ALOOKUP_index_list]>>
-    rw[LENGTH_TAKE_EQ]>>
-    gvs[LLOOKUP_cons_SUC])
-  \\ match_mp_tac IMP_filter_bitmap_EQ_SOME_NIL
-  \\ fsrw_tac[] [] \\ once_rewrite_tac [EQ_SYM_EQ]
-  \\ conj_asm1_tac THEN1 (
-      fsrw_tac[] [LENGTH_index_list,LENGTH_TAKE_EQ,MIN_DEF]
-      \\ srw_tac[][] >> decide_tac )
-  \\ fsrw_tac[] [ZIP_GENLIST] \\ pop_assum kall_tac
-  \\ `?names0 names1. names = (names0,names1)` by metis_tac[PAIR]
-  \\ gvs[cut_envs_def,AllCaseEqs(),cut_names_def]
-  \\ qmatch_goalsub_abbrev_tac`QSORT _ (toAList envs1)`
-  \\ qpat_abbrev_tac`ls = MAP _ (toAList _)`
-  \\ `!x. MEM x ls <=>
-          ?n. x = f' - 1 - (n DIV 2 - k) /\ n IN domain envs1` by (
-    fs[MEM_MAP,EXISTS_PROD,MEM_toAList,Abbr`ls`,lookup_inter_alt,domain_lookup,SUBSET_DEF,Abbr`envs1`]
-    \\ metis_tac [])
-  \\ fsrw_tac[] []
-  \\ ntac 2 (pop_assum kall_tac)
-  \\ fsrw_tac[] [MAP_FST_def,adjust_names_def]
-  \\ match_mp_tac SORTED_IMP_EQ_LISTS
-  \\ conj_tac
-  >- (
-    REWRITE_TAC[GSYM inv_image_def,sorted_map] >>
-    qmatch_abbrev_tac`SORTED R' (QSORT R ls)` >>
-    `SORTED R (QSORT R ls)` by (
-      match_mp_tac QSORT_SORTED >>
-      metis_tac[transitive_key_val_compare,total_key_val_compare] ) >>
-    match_mp_tac SORTED_weaken2>>fsrw_tac[][]>>CONJ_ASM1_TAC
-    >-
-      metis_tac[ALL_DISTINCT_MAP_FST_toAList,QSORT_PERM,ALL_DISTINCT_PERM,ALL_DISTINCT_MAP]
-    >>
-      simp[MEM_QSORT,Abbr`R`] >>
-      simp[Abbr`R'`,inv_image_def,FORALL_PROD,Abbr`ls`,MEM_toAList] >>
-      fsrw_tac[][key_val_compare_def,LET_THM]>>
-      `∀p v. lookup p envs1 = SOME v ⇒ lookup p s.locals = SOME v` by (
-        simp[Abbr`envs1`,lookup_inter_EQ])>>
-      srw_tac[][]>>fsrw_tac[][]>>res_tac>>res_tac>>
-      fsrw_tac[][EVEN_GT])
-  \\ conj_tac
-  >- (
-    ONCE_REWRITE_TAC[sorted_map] >>
-    REWRITE_TAC[GSYM inv_image_def] >>
-    match_mp_tac (MP_CANON sorted_filter) >>
-    conj_tac >- metis_tac[transitive_inv_image,transitive_GT] >>
-    ONCE_REWRITE_TAC[GSYM sorted_map] >>
-    simp[MAP_GENLIST,combinTheory.o_DEF] >>
-    ONCE_REWRITE_TAC[GSYM sorted_map] >>
-    simp[MAP_GENLIST,combinTheory.o_DEF] >>
-    qmatch_abbrev_tac`SORTED R (GENLIST g m)` >>
-    `GENLIST g m = GENLIST (λx. k + m - (x + 1)) m` by (
-      simp[LIST_EQ_REWRITE,Abbr`g`] >>
-      srw_tac[][] >>
-      qmatch_abbrev_tac`FST (EL x (index_list ls k)) = Z` >>
-      qmatch_assum_abbrev_tac`DROP nn ll = _`
-      \\ qispl_then[`nn`,`ll`]mp_tac LENGTH_DROP
-      \\ asm_simp_tac(std_ss)[Abbr`ll`,Abbr`nn`]
-      \\ simp[] >>
-      `x < LENGTH ls` by ( simp[Abbr`ls`] ) >>
-      asm_simp_tac std_ss [EL_index_list] >>
-      simp[Abbr`ls`,Abbr`Z`] ) >>
-    pop_assum SUBST1_TAC >>
-    fsrw_tac[][Abbr`R`]>>
-    fsrw_tac[][SORTED_EL_SUC]>>srw_tac[][]>>
-    `n'' < m` by DECIDE_TAC>>
-    fsrw_tac[][EL_GENLIST]>>DECIDE_TAC)
-  \\ simp[MEM_MAP,MEM_FILTER,MEM_GENLIST,PULL_EXISTS,MEM_QSORT,
-            MEM_toAList,EXISTS_PROD,FORALL_PROD,Abbr`envs1`]
-  \\ rw[]
-  \\ simp[lookup_inter_alt,domain_inter]
-  \\ fsrw_tac[][SUBSET_DEF]
-  \\ `LENGTH (TAKE f' t') = f'` by ( simp[LENGTH_TAKE_EQ] )
-  \\ srw_tac[][EQ_IMP_THM]
-  >- (
-    fsrw_tac[][domain_lookup,PULL_EXISTS]
-    \\ ONCE_REWRITE_TAC[CONJ_COMM]
-    \\ asm_exists_tac \\ simp[]
+    \\ fsrw_tac[][IS_PREFIX_APPEND]
+    \\ imp_res_tac read_bitmap_append_extra
+    \\ simp[DROP_APPEND]
+    \\ gvs[]
+    \\ ntac 2 (pop_assum kall_tac)
+    \\ conj_tac
+    >- (
+      srw_tac[][]
+      \\ imp_res_tac abs_stack_IMP_LENGTH
+      \\ Cases_on`s.handler<LENGTH s.stack`>>fsrw_tac[][]
+      \\ qpat_x_assum`is_handler_frame _`mp_tac
+      >- (simp[ADD1,EL_CONS,PRE_SUB1,LASTN_CONS])
+      \\ simp[ADD1]
+      \\ `LENGTH s.stack - s.handler = 0` by DECIDE_TAC
+      \\ simp[is_handler_frame_def])
+    \\ simp[stack_rel_aux_def]
+    \\ `∀x. s.permute x = I` by simp[FUN_EQ_THM]
+    \\ simp[list_rearrange_I]
+    \\ qmatch_assum_abbrev_tac`DROP nn ll = _`
+    \\ qispl_then[`nn`,`ll`]mp_tac LENGTH_DROP
+    \\ asm_simp_tac(std_ss)[Abbr`ll`,Abbr`nn`]
+    \\ simp[]
+    \\ fs[stack_size_rel_def]
+    \\ rpt strip_tac
+    >- (
+      qpat_x_assum`cut_envs _ _ = SOME _` mp_tac>>
+      simp[cut_envs_def,cut_names_def,AllCaseEqs()]>>
+      rw[]>>
+      gvs[ALOOKUP_toAList,lookup_inter,AllCaseEqs(),domain_lookup]>>
+      last_x_assum drule>>
+      strip_tac>>
+      first_x_assum drule>>
+      simp[]>>
+      strip_tac>>
+      DEP_REWRITE_TAC[ALOOKUP_index_list]>>
+      rw[LENGTH_TAKE_EQ]>>
+      gvs[LLOOKUP_cons_SUC])
+    \\ match_mp_tac IMP_filter_bitmap_EQ_SOME_NIL
+    \\ fsrw_tac[] [] \\ once_rewrite_tac [EQ_SYM_EQ]
+    \\ conj_asm1_tac THEN1 (
+        fsrw_tac[] [LENGTH_index_list,LENGTH_TAKE_EQ,MIN_DEF]
+        \\ srw_tac[][] >> decide_tac )
+    \\ fsrw_tac[] [ZIP_GENLIST] \\ pop_assum kall_tac
+    \\ `?names0 names1. names = (names0,names1)` by metis_tac[PAIR]
+    \\ gvs[cut_envs_def,AllCaseEqs(),cut_names_def]
+    \\ qmatch_goalsub_abbrev_tac`QSORT _ (toAList envs1)`
+    \\ qpat_abbrev_tac`ls = MAP _ (toAList _)`
+    \\ `!x. MEM x ls <=>
+            ?n. x = f' - 1 - (n DIV 2 - k) /\ n IN domain envs1` by (
+      fs[MEM_MAP,EXISTS_PROD,MEM_toAList,Abbr`ls`,lookup_inter_alt,domain_lookup,SUBSET_DEF,Abbr`envs1`]
+      \\ metis_tac [])
+    \\ fsrw_tac[] []
+    \\ ntac 2 (pop_assum kall_tac)
+    \\ fsrw_tac[] [MAP_FST_def,adjust_names_def]
+    \\ match_mp_tac SORTED_IMP_EQ_LISTS
+    \\ conj_tac
+    >- (
+      REWRITE_TAC[GSYM inv_image_def,sorted_map] >>
+      qmatch_abbrev_tac`SORTED R' (QSORT R ls)` >>
+      `SORTED R (QSORT R ls)` by (
+        match_mp_tac QSORT_SORTED >>
+        metis_tac[transitive_key_val_compare,total_key_val_compare] ) >>
+      match_mp_tac SORTED_weaken2>>fsrw_tac[][]>>CONJ_ASM1_TAC
+      >-
+        metis_tac[ALL_DISTINCT_MAP_FST_toAList,QSORT_PERM,ALL_DISTINCT_PERM,ALL_DISTINCT_MAP]
+      >>
+        simp[MEM_QSORT,Abbr`R`] >>
+        simp[Abbr`R'`,inv_image_def,FORALL_PROD,Abbr`ls`,MEM_toAList] >>
+        fsrw_tac[][key_val_compare_def,LET_THM]>>
+        `∀p v. lookup p envs1 = SOME v ⇒ lookup p s.locals = SOME v` by (
+          simp[Abbr`envs1`,lookup_inter_EQ])>>
+        srw_tac[][]>>fsrw_tac[][]>>res_tac>>res_tac>>
+        fsrw_tac[][EVEN_GT])
+    \\ conj_tac
+    >- (
+      ONCE_REWRITE_TAC[sorted_map] >>
+      REWRITE_TAC[GSYM inv_image_def] >>
+      match_mp_tac (MP_CANON sorted_filter) >>
+      conj_tac >- metis_tac[transitive_inv_image,transitive_GT] >>
+      ONCE_REWRITE_TAC[GSYM sorted_map] >>
+      simp[MAP_GENLIST,combinTheory.o_DEF] >>
+      ONCE_REWRITE_TAC[GSYM sorted_map] >>
+      simp[MAP_GENLIST,combinTheory.o_DEF] >>
+      qmatch_abbrev_tac`SORTED R (GENLIST g m)` >>
+      `GENLIST g m = GENLIST (λx. k + m - (x + 1)) m` by (
+        simp[LIST_EQ_REWRITE,Abbr`g`] >>
+        srw_tac[][] >>
+        qmatch_abbrev_tac`FST (EL x (index_list ls k)) = Z` >>
+        qmatch_assum_abbrev_tac`DROP nn ll = _`
+        \\ qispl_then[`nn`,`ll`]mp_tac LENGTH_DROP
+        \\ asm_simp_tac(std_ss)[Abbr`ll`,Abbr`nn`]
+        \\ simp[] >>
+        `x < LENGTH ls` by ( simp[Abbr`ls`] ) >>
+        asm_simp_tac std_ss [EL_index_list] >>
+        simp[Abbr`ls`,Abbr`Z`] ) >>
+      pop_assum SUBST1_TAC >>
+      fsrw_tac[][Abbr`R`]>>
+      fsrw_tac[][SORTED_EL_SUC]>>srw_tac[][]>>
+      `n'' < m` by DECIDE_TAC>>
+      fsrw_tac[][EL_GENLIST]>>DECIDE_TAC)
+    \\ simp[MEM_MAP,MEM_FILTER,MEM_GENLIST,PULL_EXISTS,MEM_QSORT,
+              MEM_toAList,EXISTS_PROD,FORALL_PROD,Abbr`envs1`]
+    \\ rw[]
+    \\ simp[lookup_inter_alt,domain_inter]
+    \\ fsrw_tac[][SUBSET_DEF]
+    \\ `LENGTH (TAKE f' t') = f'` by ( simp[LENGTH_TAKE_EQ] )
+    \\ srw_tac[][EQ_IMP_THM]
+    >- (
+      fsrw_tac[][domain_lookup,PULL_EXISTS]
+      \\ ONCE_REWRITE_TAC[CONJ_COMM]
+      \\ asm_exists_tac \\ simp[]
+      \\ first_x_assum drule >> strip_tac
+      \\ first_x_assum drule
+      \\ last_x_assum drule
+      \\ IF_CASES_TAC >- simp[]
+      \\ simp[LLOOKUP_THM,EVEN_EXISTS]
+      \\ strip_tac >> rveq
+      \\ fsrw_tac[][MULT_COMM,MULT_DIV]
+      \\ fsrw_tac[ARITH_ss][EL_CONS,PRE_SUB1]
+      \\ simp[EL_index_list] )
+    \\ fsrw_tac[][domain_lookup]
     \\ first_x_assum drule >> strip_tac
     \\ first_x_assum drule
     \\ last_x_assum drule
@@ -1566,29 +1565,27 @@ Proof
     \\ strip_tac >> rveq
     \\ fsrw_tac[][MULT_COMM,MULT_DIV]
     \\ fsrw_tac[ARITH_ss][EL_CONS,PRE_SUB1]
-    \\ simp[EL_index_list] )
-  \\ fsrw_tac[][domain_lookup]
-  \\ first_x_assum drule >> strip_tac
-  \\ first_x_assum drule
-  \\ last_x_assum drule
-  \\ IF_CASES_TAC >- simp[]
-  \\ simp[LLOOKUP_THM,EVEN_EXISTS]
-  \\ strip_tac >> rveq
-  \\ fsrw_tac[][MULT_COMM,MULT_DIV]
-  \\ fsrw_tac[ARITH_ss][EL_CONS,PRE_SUB1]
-  \\ rfs[]
-  \\ qpat_x_assum`_ = EL _ (index_list _ _)`(mp_tac o SYM)
-  \\ simp[EL_index_list] >> strip_tac >> rveq
-  \\ ONCE_REWRITE_TAC[CONJ_COMM]
-  \\ asm_exists_tac
-  \\ simp[]
-  \\ simp_tac (srw_ss()) [MULT_COMM,MULT_DIV]
+    \\ rfs[]
+    \\ qpat_x_assum`_ = EL _ (index_list _ _)`(mp_tac o SYM)
+    \\ simp[EL_index_list] >> strip_tac >> rveq
+    \\ ONCE_REWRITE_TAC[CONJ_COMM]
+    \\ asm_exists_tac
+    \\ simp[]
+    \\ simp_tac (srw_ss()) [MULT_COMM,MULT_DIV]
+  ) >>
+  fs[stack_size_rel_def] >> rw[]
+  >- (
+    rw[OPTION_MAP2_DEF,IS_SOME_EXISTS,MAX_DEF] >>
+    fs[the_eqn,stack_size_eq] >> fs[])
+  >- (
+    fs[IS_SOME_EXISTS,OPTION_MAP2_DEF,PULL_EXISTS] >> fs[] >>
+    fs[the_eqn,CaseEq"option",stack_size_eq] >>
+    rveq >> fs[])
 QED
 
-
 Triviality state_rel_set_store_0:
-  state_rel ac k 0 0 s5 t5 len ==>
-    state_rel ac k 0 0 (set_store AllocSize w s5) (set_store AllocSize w t5) len
+  state_rel ac k 0 0 s5 t5 len extra ⇒
+  state_rel ac k 0 0 (set_store AllocSize w s5) (set_store AllocSize w t5) len extra
 Proof
   rpt strip_tac
   \\ fs [state_rel_def,set_store_def,stackSemTheory.set_store_def,LET_DEF,
@@ -1683,7 +1680,7 @@ Proof
 QED
 
 Triviality IMP_enc_stack:
-  state_rel ac k 0 0 s1 t1 lens
+  state_rel ac k 0 0 s1 t1 lens 0
     ==>
     (enc_stack t1.bitmaps (DROP t1.stack_space t1.stack) =
        SOME (enc_stack s1.stack))
@@ -1999,9 +1996,12 @@ Proof
 QED
 
 Triviality gc_state_rel:
-  (gc (s1:('a,num # 'c,'ffi) wordSem$state) = SOME s2) /\ state_rel ac k 0 0 s1 (t1:('a,'c,'ffi) stackSem$state) lens  ==>
-    ?(t2:('a,'c,'ffi) stackSem$state). gc t1 = SOME t2 /\ state_rel ac k 0 0 (s2 with locals:= LN) t2 lens
-    /\ LENGTH t2.stack = LENGTH t1.stack /\ t2.stack_space = t1.stack_space
+  gc (s1:('a,num # 'c,'ffi) wordSem$state) = SOME s2 /\
+  state_rel ac k 0 0 s1 (t1:('a,'c,'ffi) stackSem$state) lens 0 ⇒
+  ?(t2:('a,'c,'ffi) stackSem$state).
+    gc t1 = SOME t2 /\
+    state_rel ac k 0 0 (s2 with locals:= LN) t2 lens 0 /\
+    LENGTH t2.stack = LENGTH t1.stack /\ t2.stack_space = t1.stack_space
 Proof
   fs [gc_def,LET_DEF]
   \\ Cases_on `s1.gc_fun (enc_stack s1.stack,s1.memory,s1.mdomain,s1.store)` \\ fs []
@@ -2021,8 +2021,7 @@ Proof
   \\ rfs [FLOOKUP_DEF] \\ rw[]
   THEN1 (fs [fmap_EXT,EXTENSION,DOMSUB_FAPPLY_THM] \\ metis_tac [])
   \\ fs [DROP_APPEND,DROP_TAKE_NIL]
-  \\ TRY(qmatch_goalsub_abbrev_tac `post_alloc_conventions _` >> metis_tac[])
-  \\ TRY(qmatch_goalsub_abbrev_tac `flat_exp_conventions _` >> metis_tac[])
+  \\ gvs[stack_size_rel_def]
   \\ metis_tac[dec_stack_stack_size]
 QED
 
@@ -2087,19 +2086,23 @@ Triviality alloc_IMP_alloc:
     (∀x. x ∈ domain (FST names) ⇒ EVEN x /\ k ≤ x DIV 2) /\
     (∀x. x ∈ domain (SND names) ⇒ EVEN x /\ k ≤ x DIV 2) /\
     1 ≤ f /\
-    state_rel ac k f f' s t5 lens /\
-    state_rel ac k 0 0 (push_env envs ^nn s with <|locals := LN; locals_size := SOME 0|>) t5 (f'::lens) /\
+    state_rel ac k f f' s t5 lens 0 /\
+    state_rel ac k 0 0 (push_env envs ^nn s with <|locals := LN; locals_size := SOME 0|>) t5 (f'::lens) 0 /\
     (cut_envs names s.locals = SOME envs) /\
     res <> SOME Error ==>
     ?t1:('a,'c,'ffi) stackSem$state res1.
       (stackSem$alloc c t5 = (res1:'a stackSem$result option,t1)) /\
       if res = NONE then
-        res1 = NONE /\ state_rel ac k f f' s1 t1 lens /\ LENGTH t1.stack = LENGTH t5.stack
-                                                   /\ t1.stack_space = t5.stack_space
+        res1 = NONE /\
+        state_rel ac k f f' s1 t1 lens 0 /\
+        LENGTH t1.stack = LENGTH t5.stack /\
+        t1.stack_space = t5.stack_space
       else
         res = SOME NotEnoughSpace /\ res1 = SOME (Halt (Word 1w)) /\
         s1.clock = t1.clock /\ s1.ffi = t1.ffi
 Proof
+  cheat
+  (*
   Cases_on `FST (alloc c names (s:('a,num # 'c,'ffi) wordSem$state)) = SOME (Error:'a result)`
   THEN1 (rpt strip_tac \\ fsrw_tac[] [] \\ rfs [])
   \\ fsrw_tac[] [alloc_alt, stackSemTheory.alloc_def]
@@ -2114,7 +2117,7 @@ Proof
   \\ rename1`pop_env x`
   \\ Cases_on `pop_env x` \\ fsrw_tac[] []
   \\ Q.MATCH_ASSUM_RENAME_TAC `pop_env s2 = SOME s3`
-  \\ `state_rel ac k f f' s3 t2 lens` by (
+  \\ `state_rel ac k f f' s3 t2 lens 0` by (
     imp_res_tac gc_s_key_eq>>
     fsrw_tac[][set_store_def]>>
     imp_res_tac push_env_pop_env_s_key_eq>>
@@ -2271,7 +2274,7 @@ Proof
   \\ drule_all FLOOKUP_SUBMAP \\ simp[]
   \\ gvs[has_space_def,AllCaseEqs(),stackSemTheory.has_space_def,get_store_def]
   \\ imp_res_tac FLOOKUP_SUBMAP \\ fsrw_tac[] []
-  \\ fsrw_tac[] [state_rel_def]
+  \\ fsrw_tac[] [state_rel_def] *)
 QED
 
 Triviality word_gc_empty_frame:
@@ -2296,19 +2299,23 @@ QED
 
 Triviality alloc_IMP_alloc2:
   (wordSem$alloc c names (s:('a,num # 'c,'ffi) wordSem$state) = (res:'a result option,s1)) ∧
-  state_rel ac k 0 0 s t lens ∧
+  state_rel ac k 0 0 s t lens 0 ∧
   domain (FST names) = {} ∧
   domain (SND names) = {} ∧
   res ≠ SOME Error ⇒
   ∃(t1:('a,'c,'ffi) stackSem$state) res1.
     (stackSem$alloc c t = (res1:'a stackSem$result option,t1)) ∧
     if res = NONE then
-      res1 = NONE ∧ state_rel ac k 0 0 s1 t1 lens /\ LENGTH t1.stack = LENGTH t.stack /\
+      res1 = NONE ∧
+      state_rel ac k 0 0 s1 t1 lens 0 /\
+      LENGTH t1.stack = LENGTH t.stack /\
       t1.stack_space = t.stack_space
     else
       res = SOME NotEnoughSpace /\ res1 = SOME (Halt (Word 1w)) ∧
       s1.clock = t1.clock /\ s1.ffi = t1.ffi
 Proof
+  cheat
+  (*
   Cases_on `FST (alloc c names (s:('a,num # 'c,'ffi) wordSem$state)) = SOME (Error:'a result)`
   THEN1 (rpt strip_tac \\ fs [] \\ rfs [])
   \\ fs [alloc_alt, stackSemTheory.alloc_def]
@@ -2367,7 +2374,7 @@ Proof
   \\ fs[dec_stack_def,CaseEq"option",CaseEq"prod",CaseEq"bool"]
   \\ fs[state_component_equality] >> rveq >> fs[]
   \\ imp_res_tac dec_stack_stack_size
-  \\ fs[]
+  \\ fs[] *)
 QED
 
 Definition compile_result_def:
@@ -2844,7 +2851,10 @@ Proof
 QED
 
 Theorem state_rel_get_var_imp:
-  state_rel ac k f f' s t lens ∧ get_var (2 * x) s = SOME v ∧ x < k ⇒ FLOOKUP t.regs x = SOME v
+  state_rel ac k f f' s t lens extra ∧
+  get_var (2 * x) s = SOME v ∧
+  x < k ⇒
+  FLOOKUP t.regs x = SOME v
 Proof
   simp[state_rel_def]
   \\ strip_tac
@@ -2857,7 +2867,7 @@ Proof
 QED
 
 Theorem state_rel_get_var_imp2:
-  state_rel ac k f f' s t lens ∧
+  state_rel ac k f f' s t lens 0 ∧
   get_var (2 * x) s = SOME v ∧
   ¬(x < k)
   ⇒
@@ -2879,8 +2889,10 @@ Proof
 QED
 
 Theorem state_rel_set_var_k[simp]:
-   (state_rel ac k f f' s (set_var (k+1) v t) lens ⇔ state_rel ac k f f' s t lens) ∧
-   (state_rel ac k f f' s (set_var k v t) lens ⇔ state_rel ac k f f' s t lens)
+   (state_rel ac k f f' s (set_var (k+1) v t) lens extra ⇔
+    state_rel ac k f f' s t lens extra) ∧
+   (state_rel ac k f f' s (set_var k v t) lens extra ⇔
+    state_rel ac k f f' s t lens extra)
 Proof
   conj_tac
   \\ simp[state_rel_def,EQ_IMP_THM,stackSemTheory.set_var_def]
@@ -2890,8 +2902,9 @@ Proof
 QED
 
 Theorem state_rel_set_var:
-    state_rel ac k f f' s t lens ∧ x < k ⇒
-    state_rel ac k f f' (set_var (2*x) v s) (set_var x v t) lens
+    state_rel ac k f f' s t lens extra ∧
+    x < k ⇒
+    state_rel ac k f f' (set_var (2*x) v s) (set_var x v t) lens extra
 Proof
   simp[state_rel_def,stackSemTheory.set_var_def,wordSemTheory.set_var_def]
   \\ strip_tac
@@ -2912,11 +2925,14 @@ Proof
 QED
 
 Theorem state_rel_set_var2:
-    state_rel ac k f f' s t lens ∧ ¬(x < k) ∧ x < f' + k ∧ st = t.stack ∧ sp = t.stack_space ⇒
-    state_rel ac k f f' (set_var (2*x) v s)
-    (t with stack := LUPDATE v (sp + (f + k − (x + 1))) st) lens
+  state_rel ac k f f' s t lens 0 ∧
+  ¬(x < k) ∧ x < f' + k ∧ st = t.stack ∧ sp = t.stack_space ⇒
+  state_rel ac k f f' (set_var (2*x) v s)
+    (t with stack := LUPDATE v (sp + (f + k − (x + 1))) st) lens 0
 Proof
-  simp[state_rel_def,stackSemTheory.set_var_def,wordSemTheory.set_var_def]
+  cheat
+  (*
+  simp[state_rel_def,stackSemTheory.set_var_def,wordSemTheory.set_var_def,stack_size_rel_def]
   \\ strip_tac
   \\ `0<f` by
       (Cases_on`f'`>>fs[]>>DECIDE_TAC)
@@ -2952,18 +2968,18 @@ Proof
   \\ simp[MULT_DIV]
   \\ ntac 2 strip_tac
   \\ rw[]
-  \\ fsrw_tac[ARITH_ss][]
+  \\ fsrw_tac[ARITH_ss][] *)
 QED
 
 Theorem wMoveSingle_thm:
-   state_rel ac k f f' s t lens ∧
+   state_rel ac k f f' s t lens 0 ∧
    (case x of NONE => get_var (k+1) t = SOME v
     | SOME x => get_var (x * 2) s = SOME v ) ∧
    (case y of SOME x => x < f' + k | _ => T)
    ⇒
    ∃t'.
      evaluate (wMoveSingle (format_var k y,format_var k x) (k,f,f'), t) = (NONE,t') ∧
-     state_rel ac k f f' (case y of NONE => s | SOME y => set_var (y*2) v s) t' lens ∧
+     state_rel ac k f f' (case y of NONE => s | SOME y => set_var (y*2) v s) t' lens 0 ∧
      (y = NONE ⇒ get_var (k+1) t' = SOME v) ∧
      (y ≠ NONE ⇒ get_var (k+1) t' = get_var (k+1) t) /\
      LENGTH t'.stack = LENGTH t.stack /\ t'.stack_space = t.stack_space
@@ -3092,7 +3108,7 @@ Theorem with_same_locals[simp] =
 
 Theorem evaluate_wMoveAux_seqsem:
    ∀ms s t r.
-   state_rel ac k f f' s t lens ∧
+   state_rel ac k f f' s t lens 0 ∧
    (∀i v. r (SOME i) = SOME v ⇔ get_var (2*i) s = SOME v) ∧
    (∀v. r NONE = SOME v ⇒ get_var (k+1) t = SOME v) ∧
    IS_SOME (get_vars (MAP ($* 2 o THE) (FILTER IS_SOME (MAP SND ms))) s) ∧
@@ -3111,7 +3127,7 @@ Theorem evaluate_wMoveAux_seqsem:
        (set_vars
          (MAP ($* 2 o THE) (FILTER IS_SOME (MAP FST (REVERSE ms))))
          (MAP THE (MAP (seqsem ms r) (FILTER IS_SOME (MAP FST (REVERSE ms)))))
-         s) t' lens /\
+         s) t' lens 0 /\
      LENGTH t'.stack = LENGTH t.stack /\ t'.stack_space = t.stack_space
 Proof
   Induct
@@ -3277,12 +3293,12 @@ QED
 
 Theorem call_dest_lemma[local]:
   ¬bad_dest_args dest args /\
-  state_rel ac k f f' (s:('a,num # 'c,'ffi) state) t lens /\
+  state_rel ac k f f' (s:('a,num # 'c,'ffi) state) t lens 0 /\
   call_dest dest args (k,f,f') = (q0,dest') /\
   get_vars args s = SOME args' ==>
   ?t4:('a,'c,'ffi) stackSem$state.
     evaluate (q0,t) = (NONE,t4) /\
-    state_rel ac k f f' s t4 lens /\
+    state_rel ac k f f' s t4 lens 0 /\
     LENGTH t4.stack = LENGTH t.stack /\
     t4.stack_space = t.stack_space /\
     !real_args prog ssize.
@@ -3683,14 +3699,14 @@ Proof
 QED
 
 Theorem wRegWrite1_thm1:
-   state_rel ac k f f' s t lens ∧
+   state_rel ac k f f' s t lens 0 ∧
    m < f' + k ∧
    (∀n.  n ≤ k ⇒
      evaluate (kont n, t) = (NONE, set_var n v t))
    ⇒
    ∃t'.
    evaluate (wRegWrite1 kont (2 * m) (k,f,f'), t) = (NONE, t') ∧
-   state_rel ac k f f' (set_var (2 * m) v s) t' lens /\
+   state_rel ac k f f' (set_var (2 * m) v s) t' lens 0 /\
    LENGTH t'.stack = LENGTH t.stack /\ t'.stack_space = t.stack_space
 Proof
   rw[wRegWrite1_def,LET_THM,TWOxDIV2]
@@ -3706,27 +3722,27 @@ Proof
 QED
 
 Theorem wRegWrite1_thm1_weak:
-   state_rel ac k f f' s t lens ∧
+   state_rel ac k f f' s t lens 0 ∧
    m < f' + k ∧
    (∀n.  n ≤ k ⇒
      evaluate (kont n, t) = (NONE, set_var n v t))
    ⇒
    ∃t'.
    evaluate (wRegWrite1 kont (2 * m) (k,f,f'), t) = (NONE, t') ∧
-   state_rel ac k f f' (set_var (2 * m) v s) t' lens
+   state_rel ac k f f' (set_var (2 * m) v s) t' lens 0
 Proof
   metis_tac[wRegWrite1_thm1]
 QED
 
 Theorem wRegWrite1_thm2:
-   state_rel ac k f f' s t lens ∧
+   state_rel ac k f f' s t lens 0 ∧
    m < f' + k ∧
    (∀n.  n ≤ k ⇒
      evaluate (kont n, t) = (NONE, set_var 0 v' (set_var n v t)))
    ⇒
    ∃t'.
    evaluate (wRegWrite1 kont (2 * m) (k,f,f'), t) = (NONE, t') ∧
-   state_rel ac k f f' (set_var 0 v' (set_var (2 * m) v s)) t' lens /\
+   state_rel ac k f f' (set_var 0 v' (set_var (2 * m) v s)) t' lens 0 /\
    LENGTH t'.stack = LENGTH t.stack /\ t'.stack_space = t.stack_space
 Proof
   rw[wRegWrite1_def,LET_THM,TWOxDIV2]
@@ -3774,16 +3790,15 @@ Theorem wRegWrite1_thm6 =
   |> Q.INST [`t`|-> `set_var v1 v2 (set_var v3 v4 t)`]
   |> PURE_REWRITE_RULE[wordPropsTheory.set_var_const,set_var_const];
 
-
 Theorem wRegWrite2_thm1:
-   state_rel ac k f f' s t lens ∧
+   state_rel ac k f f' s t lens 0 ∧
    m < f' + k ∧
    (∀n.  n ≤ k+1 ⇒
      evaluate (kont n, t) = (NONE, set_var n v t))
    ⇒
    ∃t'.
    evaluate (wRegWrite2 kont (2 * m) (k,f,f'), t) = (NONE, t') ∧
-   state_rel ac k f f' (set_var (2 * m) v s) t' lens
+   state_rel ac k f f' (set_var (2 * m) v s) t' lens 0
 Proof
   rw[wRegWrite2_def,LET_THM,TWOxDIV2]
   >- ( metis_tac[ state_rel_set_var, LESS_OR_EQ] )
@@ -3798,11 +3813,11 @@ Proof
 QED
 
 Theorem state_rel_mem_store:
-   state_rel ac k f f' s t lens ∧
+   state_rel ac k f f' s t lens extra ∧
    mem_store a b s = SOME s' ⇒
    ∃t'.
      mem_store a b t = SOME t' ∧
-     state_rel ac k f f' s' t' lens
+     state_rel ac k f f' s' t' lens extra
 Proof
   simp[state_rel_def,stackSemTheory.mem_store_def,wordSemTheory.mem_store_def]
   \\ strip_tac \\ rveq \\ simp[] \\ metis_tac[]
@@ -3903,21 +3918,23 @@ QED
 Theorem wStackLoad_thm1:
    wReg1 (2 * n1) (k,f,f') = (l,n2) ∧
    get_var (2*n1) (s:('a,num # 'c,'ffi)wordSem$state) = SOME x ∧
-   state_rel ac k f f' s t lens ∧
+   state_rel ac k f f' s t lens extra ∧
    (n1 < k ⇒ ∃t'. evaluate (kont n1, t) = (NONE, t') ∧
-                  state_rel ac k f f' s' t' lens /\
+                  state_rel ac k f f' s' t' lens extra /\
                   LENGTH t'.stack = LENGTH t.stack /\
                   t'.stack_space = t.stack_space) ∧
    (¬(n1 < k) ⇒
     ∃t'. evaluate (kont k,
                    set_var k (EL (t.stack_space + (f+k-(n1+1))) t.stack) t) =
          (NONE, t') ∧
-         state_rel ac k f f' s' t' lens /\ LENGTH t'.stack = LENGTH t.stack /\
+         state_rel ac k f f' s' t' lens extra /\
+         LENGTH t'.stack = LENGTH t.stack /\
          t'.stack_space = t.stack_space)
    ⇒
    ∃t'.
      evaluate (wStackLoad l (kont n2),t) = (NONE,t') ∧
-     state_rel ac k f f' s' t' lens  /\ LENGTH t'.stack = LENGTH t.stack /\
+     state_rel ac k f f' s' t' lens extra /\
+     LENGTH t'.stack = LENGTH t.stack /\
      t'.stack_space = t.stack_space
 Proof
   simp[wReg1_def,TWOxDIV2]
@@ -3933,14 +3950,16 @@ QED
 Theorem wStackLoad_thm1_weak:
    wReg1 (2 * n1) (k,f,f') = (l,n2) ∧
    get_var (2*n1) (s:('a,num # 'c,'ffi)state) = SOME x ∧
-   state_rel ac k f f' s t lens ∧
-   (n1 < k ⇒ ∃t'. evaluate (kont n1, t) = (NONE, t') ∧ state_rel ac k f f' s' t' lens) ∧
+   state_rel ac k f f' s t lens extra ∧
+   (n1 < k ⇒
+     ∃t'. evaluate (kont n1, t) = (NONE, t') ∧
+     state_rel ac k f f' s' t' lens extra) ∧
    (¬(n1 < k) ⇒ ∃t'. evaluate (kont k, set_var k (EL (t.stack_space + (f+k-(n1+1))) t.stack) t) = (NONE, t')
-    ∧ state_rel ac k f f' s' t' lens)
+    ∧ state_rel ac k f f' s' t' lens extra)
   ⇒
    ∃t'.
      evaluate (wStackLoad l (kont n2),t) = (NONE,t') ∧
-     state_rel ac k f f' s' t' lens
+     state_rel ac k f f' s' t' lens extra
 Proof
   simp[wReg1_def,TWOxDIV2]
   \\ rw[] \\ rw[wStackLoad_def] \\ fs[]
@@ -3955,16 +3974,19 @@ QED
 Theorem wStackLoad_thm2:
    wReg2 (2 * n1) (k,f,f') = (l,n2) ∧
    get_var (2*n1) (s:('a,num # 'c,'ffi)state) = SOME x ∧
-   state_rel ac k f f' s t lens ∧
-   (n1 < k ⇒ ∃t'. evaluate (kont n1, t) = (NONE, t') ∧ state_rel ac k f f' s' t' lens /\ LENGTH t'.stack = LENGTH t.stack /\ t'.stack_space = t.stack_space) ∧
+   state_rel ac k f f' s t lens extra ∧
+   (n1 < k ⇒ ∃t'. evaluate (kont n1, t) = (NONE, t') ∧
+     state_rel ac k f f' s' t' lens extra /\
+     LENGTH t'.stack = LENGTH t.stack /\ t'.stack_space = t.stack_space) ∧
    (¬(n1 < k) ⇒ ∃t'. evaluate (kont (k+1), set_var (k+1) (EL (t.stack_space + (f+k-(n1+1))) t.stack) t) = (NONE, t')
-    ∧ state_rel ac k f f' s' t' lens /\ LENGTH t'.stack = LENGTH t.stack /\
+    ∧ state_rel ac k f f' s' t' lens extra /\ LENGTH t'.stack = LENGTH t.stack /\
     t'.stack_space = t.stack_space)
   ⇒
    ∃t'.
      evaluate (wStackLoad l (kont n2),t) = (NONE,t') ∧
-     state_rel ac k f f' s' t' lens /\ LENGTH t'.stack = LENGTH t.stack /\
-    t'.stack_space = t.stack_space
+     state_rel ac k f f' s' t' lens extra /\
+     LENGTH t'.stack = LENGTH t.stack /\
+     t'.stack_space = t.stack_space
 Proof
   simp[wReg2_def,TWOxDIV2]
   \\ rw[] \\ rw[wStackLoad_def] \\ fs[]
@@ -3979,14 +4001,15 @@ QED
 Theorem wStackLoad_thm2_weak:
    wReg2 (2 * n1) (k,f,f') = (l,n2) ∧
    get_var (2*n1) (s:('a,num # 'c,'ffi)state) = SOME x ∧
-   state_rel ac k f f' s t lens ∧
-   (n1 < k ⇒ ∃t'. evaluate (kont n1, t) = (NONE, t') ∧ state_rel ac k f f' s' t' lens) ∧
+   state_rel ac k f f' s t lens extra ∧
+   (n1 < k ⇒ ∃t'. evaluate (kont n1, t) = (NONE, t') ∧
+     state_rel ac k f f' s' t' lens extra) ∧
    (¬(n1 < k) ⇒ ∃t'. evaluate (kont (k+1), set_var (k+1) (EL (t.stack_space + (f+k-(n1+1))) t.stack) t) = (NONE, t')
-    ∧ state_rel ac k f f' s' t' lens)
+    ∧ state_rel ac k f f' s' t' lens extra)
   ⇒
    ∃t'.
      evaluate (wStackLoad l (kont n2),t) = (NONE,t') ∧
-     state_rel ac k f f' s' t' lens
+     state_rel ac k f f' s' t' lens extra
 Proof
   simp[wReg2_def,TWOxDIV2]
   \\ rw[] \\ rw[wStackLoad_def] \\ fs[]
@@ -4044,7 +4067,7 @@ Theorem word_exp_thm1:
    ∀s e x. word_exp s e = SOME (Word x) ∧
    every_var_exp is_phy_var e ∧
    DIV2 (max_var_exp e) < k ∧
-   state_rel ac k f f' s t lens ⇒
+   state_rel ac k f f' s t lens extra ⇒
    word_exp t (map_var DIV2 e) = SOME x
 Proof
   ho_match_mp_tac word_exp_ind
@@ -4127,7 +4150,7 @@ QED
 
 Theorem word_exp_thm2:
    ∀s e x. word_exp s e = SOME (Word x) ∧
-   state_rel ac k f f' s t lens ∧
+   state_rel ac k f f' s t lens 0 ∧
    every_var_exp ($= (2 * v)) e ∧
    ¬(v < k) ⇒
    word_exp (set_var k (EL (t.stack_space + (f + k - (v + 1))) t.stack) t) (map_var (K k) e) = SOME x
@@ -4170,7 +4193,7 @@ QED
 
 Theorem word_exp_thm3:
    ∀s e x. word_exp s e = SOME (Word x) ∧
-   state_rel ac k f f' s t lens ∧
+   state_rel ac k f f' s t lens 0 ∧
    every_var_exp (λx. x = 2*v1 ∨ x = 2*v2) e ∧
    v1 < k ∧ ¬(v2 < k)
    ⇒
@@ -4216,7 +4239,7 @@ QED
 
 Theorem word_exp_thm4:
    ∀s e x. word_exp s e = SOME (Word x) ∧
-   state_rel ac k f f' s t lens ∧
+   state_rel ac k f f' s t lens 0 ∧
    every_var_exp (λx. x = 2*v1 ∨ x = 2*v2) e ∧
    v1 < k ∧ ¬(v2 < k)
    ⇒
@@ -4262,7 +4285,7 @@ QED
 
 Theorem word_exp_thm5:
    ∀s e x. word_exp s e = SOME (Word x) ∧
-   state_rel ac k f f' s t lens ∧
+   state_rel ac k f f' s t lens 0 ∧
    every_var_exp (λx. x = 2*v1 ∨ x = 2*v2) e ∧
    ¬(v1 < k) ∧ ¬(v2 < k)
    ⇒
@@ -4309,7 +4332,7 @@ QED
 
 Theorem word_exp_thm6:
    ∀s e x. word_exp s e = SOME (Word x) ∧
-   state_rel ac k f f' s t lens ∧
+   state_rel ac k f f' s t lens 0 ∧
    e = Op b [Var (2 * v1); Var (2 * v1)] ∧
    ¬(v1 < k)
    ⇒
@@ -4337,8 +4360,8 @@ Proof
 QED
 
 Theorem state_rel_with_memory:
-   state_rel ac k f f' s t lens ⇒
-   state_rel ac k f f' (s with memory := m) (t with memory := m) lens
+   state_rel ac k f f' s t lens extra ⇒
+   state_rel ac k f f' (s with memory := m) (t with memory := m) lens extra
 Proof
   simp[state_rel_def]
   \\ strip_tac \\ simp[]
@@ -4352,15 +4375,15 @@ Proof
 QED
 
 Theorem state_rel_get_fp_var:
-   state_rel ac k f f' s t lens ⇒
+   state_rel ac k f f' s t lens extra ⇒
   get_fp_var n s = get_fp_var n t
 Proof
   fs[state_rel_def,get_fp_var_def,stackSemTheory.get_fp_var_def]
 QED
 
 Theorem state_rel_set_fp_var:
-   state_rel ac k f f' s t lens ⇒
-  state_rel ac k f f' (set_fp_var n v s) (set_fp_var n v t) lens
+  state_rel ac k f f' s t lens extra ⇒
+  state_rel ac k f f' (set_fp_var n v s) (set_fp_var n v t) lens extra
 Proof
   fs[state_rel_def,set_fp_var_def,stackSemTheory.set_fp_var_def]>>rw[]>>
   metis_tac[]
@@ -4372,13 +4395,15 @@ Theorem evaluate_wInst:
    every_var_inst is_phy_var i ∧
    max_var_inst i < 2 * f' + 2 * k ∧
    inst_arg_convention i ∧
-   state_rel ac k f f' s t lens
+   state_rel ac k f f' s t lens 0
   ⇒
    ∃t'.
      evaluate (wInst i (k,f,f'), t) = (NONE,t') ∧
-     state_rel ac k f f' s' t' lens /\
+     state_rel ac k f f' s' t' lens 0 /\
      LENGTH t'.stack = LENGTH t.stack /\ t'.stack_space = t.stack_space
 Proof
+  cheat
+  (*
   simp[inst_def]
   \\ rpt gen_tac
   \\ BasicProvers.TOP_CASE_TAC
@@ -5076,12 +5101,12 @@ Proof
     >>
       every_case_tac>>fs[stackSemTheory.evaluate_def,stackSemTheory.inst_def]>>
       imp_res_tac state_rel_get_fp_var>>
-      rw[]>>fs[state_rel_set_fp_var,set_fp_var_stack])
+      rw[]>>fs[state_rel_set_fp_var,set_fp_var_stack]) *)
 QED
 
 Theorem state_rel_set_store:
-   state_rel ac k f f' s t lens ∧ v ≠ Handler ⇒
-   state_rel ac k f f' (set_store v x s) (set_store v x t) lens
+   state_rel ac k f f' s t lens extra ∧ v ≠ Handler ⇒
+   state_rel ac k f f' (set_store v x s) (set_store v x t) lens extra
 Proof
   simp[state_rel_def]
   \\ strip_tac
@@ -5166,11 +5191,11 @@ Triviality evaluate_wStackLoad_wReg1:
   wReg1 r (k,f,f') = (x ,r') ∧
   EVEN r ∧
   get_var r (s:('a,num # 'c,'ffi)state) = SOME (Word c) ∧
-  state_rel ac k f f' s t lens ⇒
+  state_rel ac k f f' s t lens 0 ⇒
   ∃t':('a,'c,'ffi) stackSem$state.
   evaluate(wStackLoad x Skip,t) = (NONE,t') ∧
   t.clock = t'.clock ∧
-  state_rel ac k f f' s t' lens ∧
+  state_rel ac k f f' s t' lens 0 ∧
   LENGTH t'.stack = LENGTH t.stack /\ t'.stack_space = t.stack_space /\
   r' ≠ k+1 ∧
   get_var r' t' = SOME (Word c)
@@ -5203,11 +5228,11 @@ Triviality evaluate_wStackLoad_wReg2:
   wReg2 r (k,f,f') = (x ,r') ∧
   EVEN r ∧
   get_var r (s:('a,num # 'c,'ffi)state) = SOME (Word c) ∧
-  state_rel ac k f f' s t lens ⇒
+  state_rel ac k f f' s t lens 0 ⇒
   ∃t':('a,'c,'ffi) stackSem$state.
   evaluate(wStackLoad x Skip,t) = (NONE,t') ∧
   t.clock = t'.clock ∧
-  state_rel ac k f f' s t' lens ∧
+  state_rel ac k f f' s t' lens 0 ∧
   LENGTH t'.stack = LENGTH t.stack /\ t'.stack_space = t.stack_space /\
   (∀r. r ≠ k+1 ⇒ get_var r t' = get_var r t) ∧
   get_var r' t' = SOME (Word c)
@@ -5287,7 +5312,7 @@ Proof
 QED
 
 Triviality state_rel_IMP_LENGTH:
-  state_rel ac k f f' s t lens ⇒
+  state_rel ac k f f' s t lens extra ⇒
   LENGTH lens = LENGTH s.stack
 Proof
   fs[state_rel_def,stack_rel_def,LET_THM]>>rw[]>>
@@ -5482,9 +5507,10 @@ Proof
   simp[]
 QED
 
+(* TODO: maybe extra = 0 *)
 Triviality evaluate_PushHandler:
   3 ≤ t.stack_space ∧
-  state_rel ac k 0 0 (push_env x' NONE s with <|locals:=LN; locals_size:=SOME 0|>) t (f'::lens) ∧
+  state_rel ac k 0 0 (push_env x' NONE s with <|locals:=LN; locals_size:=SOME 0|>) t (f'::lens) extra ∧
   loc_check t.code (x''2,x''3) ⇒
   ∃t':('a,'c,'ffi)stackSem$state.
   evaluate(PushHandler (x''2:num) (x''3:num) (k,f:num,f'),t) = (NONE,t') ∧
@@ -5495,8 +5521,10 @@ Triviality evaluate_PushHandler:
   (∀i. i ≠ k ⇒ get_var i t' = get_var i t) ∧
   t'.stack_space +3 = t.stack_space ∧
   LENGTH t'.stack = LENGTH t.stack ∧
-  state_rel ac k 0 0 (push_env x' (SOME (x''0,x''1:'a wordLang$prog,x''2,x''3)) s with <|locals:=LN; locals_size:=SOME 0|>) t' (f'::lens)
+  state_rel ac k 0 0 (push_env x' (SOME (x''0,x''1:'a wordLang$prog,x''2,x''3)) s with <|locals:=LN; locals_size:=SOME 0|>) t' (f'::lens) extra
 Proof
+  cheat
+  (*
   rw[]>>
   `t.use_stack ∧ t.use_store ∧ t.stack_space -3 < LENGTH t.stack ∧ ∃h. FLOOKUP t.store Handler = SOME h` by
     (fs[state_rel_def,flookup_thm]>>
@@ -5564,11 +5592,13 @@ Proof
   `SUC (LENGTH s.stack) - (s.handler+1) = SUC(LENGTH s.stack - (s.handler+1))` by DECIDE_TAC>>
   fs[handler_val_def,GSYM ADD1]>>
   rw[]>>
-  simp[LASTN_CONS]
+  simp[LASTN_CONS] *)
 QED
 
+(* TODO: maybe extra = 0 *)
 Theorem evaluate_PopHandler:
-  state_rel ac k 0 0 r t1 (f'::lens) ∧ pop_env r = SOME x'' /\
+  state_rel ac k 0 0 r t1 (f'::lens) extra ∧
+  pop_env r = SOME x'' /\
   s_key_eq (call_env q r'
              (push_env env (SOME (2,handler1,handler2,handler3))
                 s)).stack r.stack /\
@@ -5585,11 +5615,13 @@ Theorem evaluate_PopHandler:
   ⇒
   ∃t':('a,'c,'ffi)stackSem$state.
   evaluate(PopHandler (k,f,f') Skip,t1) = (NONE,t') ∧
-  state_rel ac k f f' (set_var 2 w0 x'') t' lens ∧
+  state_rel ac k f f' (set_var 2 w0 x'') t' lens extra ∧
   x''.handler = s.handler /\
   LENGTH t'.stack = LENGTH t1.stack /\
   t'.stack_space = t1.stack_space + 3
 Proof
+  cheat
+  (*
   rpt strip_tac >>
   fs[state_rel_def,stackSemTheory.evaluate_def,PopHandler_def,pop_env_def,
      CaseEq "list", CaseEq "stack_frame", CaseEq "prod", CaseEq "option",
@@ -5618,7 +5650,7 @@ Proof
   fsrw_tac[][lookup_insert,convs_def]>>
   IF_CASES_TAC >- rw[] >>
   strip_tac >> res_tac >>
-  metis_tac[]
+  metis_tac[] *)
 QED
 
 Triviality evaluate_PushHandler_clock:
@@ -5673,7 +5705,7 @@ Proof
 QED
 
 Triviality state_rel_code_domain:
-  state_rel ac k f f' s t lens ⇒
+  state_rel ac k f f' s t lens extra ⇒
   domain s.code ⊆ domain t.code
 Proof
   strip_tac>>fs[state_rel_def,SUBSET_DEF,domain_lookup,EXISTS_PROD]>>
@@ -5809,7 +5841,7 @@ val goal = ``
    λ(prog:'a wordLang$prog,s:('a,num # 'c,'ffi) wordSem$state).
      ∀k f f' res s1 t bs n bs' n' sprog lens.
      (wordSem$evaluate (prog,s) = (res,s1)) /\ res <> SOME Error /\
-     state_rel ac k f f' s t lens /\
+     state_rel ac k f f' s t lens 0 /\
      post_alloc_conventions k prog /\
      flat_exp_conventions prog /\
      comp ac prog (bs,n) (k,f,f') = (sprog, (bs',n')) /\
@@ -5825,8 +5857,9 @@ val goal = ``
             the (s1.stack_limit + 1) s1.stack_max > s1.stack_limit
        else
          case res of
-         | NONE => state_rel ac k f f' s1 t1 lens
-         | SOME (Result _ ys) => state_rel ac k 0 0 s1 t1 lens /\
+         | NONE => state_rel ac k f f' s1 t1 lens 0
+         | SOME (Result _ ys) =>
+            state_rel ac k 0 0 s1 t1 lens (LENGTH ys - (k - 1)) /\
             (*
               list positions:  0 1 2 3 ... k-2 k-1 k  k+1 ...
               registers:       1 2 3 4 ... k-1
@@ -5837,7 +5870,8 @@ val goal = ``
             (LLOOKUP (DROP t1.stack_space t1.stack) (LENGTH ys - (i + 1)) = SOME (EL i ys))))
          | SOME (Exception _ y) =>
            ∃cs.
-           state_rel ac k 0 0 (push_locals cs s1) t1 (LASTN (s.handler+1) lens) /\ FLOOKUP t1.regs 1 = SOME y
+           state_rel ac k 0 0 (push_locals cs s1) t1 (LASTN (s.handler+1) lens) 0 /\
+           FLOOKUP t1.regs 1 = SOME y
          | SOME _ => s1.ffi = t1.ffi /\ s1.clock = t1.clock``
 
 local
@@ -5895,7 +5929,10 @@ Proof
     \\ `t5.use_alloc` by fs [state_rel_def] \\ fs [convs_def]
     \\ Cases_on `alloc c t5` \\ fs []
     \\ rename1 `alloc c t5 = (res1,t1)` \\ fs []
-    \\ drule alloc_IMP_alloc \\ impl_tac >- (fs[])
+    \\ drule alloc_IMP_alloc
+    \\ impl_tac >- (
+      fs[]
+      )
     \\ fs [] \\ REPEAT STRIP_TAC
     \\ fs [] \\ Cases_on `res = NONE` \\ fs []
     \\ fs[state_rel_def])>>
@@ -6288,7 +6325,7 @@ Proof
   \\ strip_tac
   \\ qhdtm_x_assum`state_rel`mp_tac
   \\ rveq
-  \\ qmatch_abbrev_tac`_ _ _ _ a _ _ ⇒ _ _ _ _ b _ _`
+  \\ qmatch_abbrev_tac`state_rel _ _ _ _ a _ _ _ ⇒ state_rel _ _ _ _ b _ _ _`
   \\ `a = b` suffices_by rw[]
   \\ simp[Abbr`a`,Abbr`b`]
   \\ qpat_abbrev_tac`ls = FILTER A B`
@@ -6481,7 +6518,7 @@ Proof
   \\ ‘t.use_store’ by fs [state_rel_def]
   THEN1
    (qmatch_goalsub_abbrev_tac `wRegWrite1 kont (2 * m)`
-    \\ qmatch_goalsub_abbrev_tac `state_rel _ _ _ _ (set_var _ v _)`
+    \\ qmatch_goalsub_abbrev_tac `state_rel _ _ _ _ (set_var _ v _) _ _ _`
     \\ drule_then(qspecl_then [`v`,`m`,`kont`] mp_tac) (GEN_ALL wRegWrite1_thm1)
     \\ unabbrev_all_tac
     \\ fs[wordLangTheory.max_var_def,GSYM LEFT_ADD_DISTRIB]
@@ -6493,9 +6530,9 @@ Proof
     \\ ‘get_var (2 * m') s = SOME (Word x)’ by fs [get_var_def]
     \\ imp_res_tac state_rel_get_var_imp \\ fs [])
   \\ qmatch_goalsub_abbrev_tac `wRegWrite1 kont (2 * m)`
-  \\ qmatch_goalsub_abbrev_tac `state_rel _ _ _ _ (set_var _ v _)`
+  \\ qmatch_goalsub_abbrev_tac `state_rel _ _ _ _ (set_var _ v _) _ _ _`
   \\ qmatch_goalsub_abbrev_tac ‘_,set_var _ kval _’
-  \\ ‘state_rel ac k f f' s (set_var k kval t) lens’ by fs []
+  \\ ‘state_rel ac k f f' s (set_var k kval t) lens 0’ by fs []
   \\ drule_then(qspecl_then [`v`,`m`,`kont`] mp_tac) (GEN_ALL wRegWrite1_thm1)
   \\ unabbrev_all_tac
   \\ fs[wordLangTheory.max_var_def,GSYM LEFT_ADD_DISTRIB]
@@ -6627,12 +6664,24 @@ Proof
       state_rel_def] >> METIS_TAC[]) \\
     fs[] \\
     CONJ_TAC
-    >- (fs[state_rel_def,flush_state_def] \\
-        CONJ_TAC >- METIS_TAC[] \\
-        CONJ_TAC >- cheat \\
-        CONJ_TAC >- cheat \\
-        CONJ_TAC >- cheat \\
-        simp[lookup_def]) \\
+    >- (
+      fs[state_rel_def,flush_state_def] \\
+      CONJ_TAC >- METIS_TAC[] \\
+      CONJ_TAC >- (
+        fs[stack_size_rel_def]>>rw[]
+        >- (
+          gvs[skip_free_def,num_stack_ret_def]>>
+          (* should be provable with appropriate bounds and cancellation *)
+          cheat)
+        >- (
+          (* should be provable with appropriate bounds and cancellation *)
+          PURE_REWRITE_TAC[skip_free_def,num_stack_ret_def]>>
+          cheat) )>>
+      CONJ_TAC >- (
+        simp[skip_free_def,num_stack_ret_def]>>
+        (* cancellation of the sub terms (f - .. + ..) *)
+        cheat)>>
+      simp[lookup_def]) \\
     rpt strip_tac \\
     `get_var (EL i ms) s = SOME (EL i ys)`
        by(
@@ -6670,15 +6719,16 @@ Proof
        qpat_x_assum `ms = GENLIST _ _` SUBST_ALL_TAC \\
        fs[list_max_GENLIST_evens2]) \\
     fs[])
-  >- (fs[wStackLoad_def,stackSemTheory.evaluate_def] \\
-  `t.use_stack /\ (t.stack_space + (f + k − (n DIV 2 + 1))) < LENGTH t.stack`
-   by (fs [state_rel_def,get_var_def,LET_DEF]
-    \\ res_tac \\ qpat_x_assum `!x.bbb` (K ALL_TAC) \\ rfs []
-    \\ fs [stackSemTheory.get_var_def]
-    \\ imp_res_tac LLOOKUP_TAKE_IMP
-    \\ fs [LLOOKUP_DROP] \\ fs [LLOOKUP_THM] \\ rw[]
-    \\ rfs[EL_TAKE]) \\
-  fs[] \\
+  >- (
+    fs[wStackLoad_def,stackSemTheory.evaluate_def] \\
+    `t.use_stack /\ (t.stack_space + (f + k − (n DIV 2 + 1))) < LENGTH t.stack` by (
+      fs [state_rel_def,get_var_def,LET_DEF]
+      \\ res_tac \\ qpat_x_assum `!x.bbb` (K ALL_TAC) \\ rfs []
+      \\ fs [stackSemTheory.get_var_def]
+      \\ imp_res_tac LLOOKUP_TAKE_IMP
+      \\ fs [LLOOKUP_DROP] \\ fs [LLOOKUP_THM] \\ rw[]
+      \\ rfs[EL_TAKE]) \\
+    fs[] \\
     DEP_REWRITE_TAC[evaluate_SeqStackFree] \\
     CONJ_ASM1_TAC >- (fs []) \\
     fs [stackSemTheory.evaluate_def] \\
@@ -6693,12 +6743,23 @@ Proof
     \\ rfs[EL_TAKE]) \\
     fs[] \\
     CONJ_TAC
-    >- (fs[state_rel_def,flush_state_def] \\
-        CONJ_TAC >- METIS_TAC[] \\
-        CONJ_TAC >- cheat \\
-        CONJ_TAC >- cheat \\
-        CONJ_TAC >- cheat \\
-        simp[lookup_def]) \\
+    >- (
+      fs[state_rel_def,flush_state_def] \\
+      CONJ_TAC >- metis_tac[] \\
+      CONJ_TAC >- (
+        fs[stack_size_rel_def]>>rw[]
+        >- (
+          gvs[skip_free_def,num_stack_ret_def]>>
+          (* should be provable with appropriate bounds and cancellation *)
+          cheat)
+        >- (
+          (* should be provable with appropriate bounds and cancellation *)
+          PURE_REWRITE_TAC[skip_free_def,num_stack_ret_def]>>
+          cheat) )
+      CONJ_TAC >- (
+        simp[skip_free_def,num_stack_ret_def]>>
+        cheat) \\
+      simp[lookup_def]) \\
     simp[stackSemTheory.set_var_def,FLOOKUP_UPDATE] \\
     rpt strip_tac \\
     `get_var (EL i ms) s = SOME (EL i ys)`
